src/Lean/Meta/Tactic/Grind/Arith/Cutsat.lean
@@ -16,6 +16,7 @@ import Lean.Meta.Tactic.Grind.Arith.Cutsat.Var
 import Lean.Meta.Tactic.Grind.Arith.Cutsat.EqCnstr
 import Lean.Meta.Tactic.Grind.Arith.Cutsat.SearchM
 import Lean.Meta.Tactic.Grind.Arith.Cutsat.Model
+import Lean.Meta.Tactic.Grind.Arith.Cutsat.DivMod
 
 namespace Lean
 
@@ -56,5 +57,7 @@ builtin_initialize registerTraceClass `grind.debug.cutsat.backtrack
 builtin_initialize registerTraceClass `grind.debug.cutsat.search
 builtin_initialize registerTraceClass `grind.debug.cutsat.cooper
 builtin_initialize registerTraceClass `grind.debug.cutsat.conflict
+builtin_initialize registerTraceClass `grind.debug.cutsat.assign
+builtin_initialize registerTraceClass `grind.debug.cutsat.subst
 
 end Lean
