src/Lean/Meta/Tactic/Grind/Arith/Cutsat/Search.lean
@@ -86,6 +86,7 @@ where
       modify' fun s => { s with assignment := s.assignment.set x 0 }
       let some v ← c.p.eval? | c.throwUnexpected
       let v := (-v) / a
+      trace[grind.debug.cutsat.assign] "{← getVar x}, {← c.pp}, {v}"
       traceAssignment x v
       modify' fun s => { s with assignment := s.assignment.set x v }
       go xs
